theories/language/proofmode.v
@@ -95,8 +95,6 @@ Section zebre_G.
 
   Lemma tac_wp_equal Δ Δ' K v1 v2 E Φ :
     MaybeIntoLaterNEnvs 1 Δ Δ' →
-    ValPhysical v1 →
-    ValPhysical v2 →
     ( val_neq v1 v2 →
       envs_entails Δ' (WP fill K #false @ E {{ Φ }})
     ) →
@@ -105,7 +103,7 @@ Section zebre_G.
     ) →
     envs_entails Δ (WP fill K (v1 = v2) @ E {{ Φ }}).
   Proof.
-    rewrite envs_entails_unseal => HΔ Hv1 Hv2 Hfail Hsuc.
+    rewrite envs_entails_unseal => HΔ Hfail Hsuc.
     rewrite into_laterN_env_sound -wp_bind -wp_equal //.
     apply bi.later_mono, bi.and_intro.
     all: rewrite bi.pure_wand_forall // -bi.forall_intro //.
@@ -232,8 +230,6 @@ Section zebre_G.
   Lemma tac_wp_cas Δ Δ' Δ'' id p K l dq v v1 v2 E Φ :
     MaybeIntoLaterNEnvs 1 Δ Δ' →
     envs_lookup_delete true id Δ' = Some (p, l ↦{dq} v, Δ'')%I →
-    ValPhysical v →
-    ValPhysical v1 →
     ( val_neq v v1 →
       envs_entails Δ' (WP fill K #false @ E {{ Φ }})
     ) →
@@ -249,7 +245,7 @@ Section zebre_G.
     end →
     envs_entails Δ (WP fill K (Cas #l v1 v2) @ E {{ Φ }}).
   Proof.
-    rewrite envs_entails_unseal. intros HΔ (Hlookup & ->)%envs_lookup_delete_Some Hv Hv1 Hfail Hsuc1 Hsuc2.
+    rewrite envs_entails_unseal. intros HΔ (Hlookup & ->)%envs_lookup_delete_Some Hfail Hsuc1 Hsuc2.
     destruct (envs_app _ _ _) as [Δ''' |] eqn:HΔ'''; last done.
     rewrite into_laterN_env_sound -wp_bind //=.
     iIntros "HΔ'".
@@ -274,8 +270,6 @@ Section zebre_G.
   Lemma tac_wp_cas_suc Δ Δ' id K l lit lit1 v2 E Φ :
     MaybeIntoLaterNEnvs 1 Δ Δ' →
     envs_lookup id Δ' = Some (false, l ↦ #lit)%I →
-    literal_physical lit →
-    literal_physical lit1 →
     lit = lit1 →
     match envs_simple_replace id false (Esnoc Enil id (l ↦ v2)) Δ' with
     | Some Δ'' =>
@@ -285,7 +279,7 @@ Section zebre_G.
     end →
     envs_entails Δ (WP fill K (Cas #l #lit1 v2) @ E {{ Φ }}).
   Proof.
-    rewrite envs_entails_unseal. intros HΔ Hlookup Hlit Hlit1 -> HΔ'.
+    rewrite envs_entails_unseal. intros HΔ Hlookup -> HΔ'.
     destruct (envs_simple_replace _ _ _ _) as [Δ'' |] eqn:HΔ''; last done.
     rewrite into_laterN_env_sound -wp_bind envs_simple_replace_sound //= HΔ'.
     iIntros "(Hl & H)".
@@ -440,9 +434,6 @@ Tactic Notation "wp_bind" open_constr(e_foc) :=
     ]
   ).
 
-#[local] Ltac solve_val_physical :=
-  try (fast_done || tc_solve).
-
 Tactic Notation "wp_equal" "as" simple_intropattern(Hfail) "|" simple_intropattern(Hsuc) :=
   wp_pures;
   wp_start ltac:(fun e =>
@@ -453,8 +444,6 @@ Tactic Notation "wp_equal" "as" simple_intropattern(Hfail) "|" simple_intropatte
     | fail 1 "wp_equal: cannot find 'Equal' in" e
     ];
     [ tc_solve
-    | solve_val_physical
-    | solve_val_physical
     | intros Hfail;
       wp_finish
     | intros Hsuc;
@@ -622,8 +611,6 @@ Tactic Notation "wp_cas" "as" simple_intropattern(Hfail) "|" simple_intropattern
       [ iAssumptionCore
       | fail 1 "wp_cas: cannot find" l "↦ ?"
       ]
-    | solve_val_physical
-    | solve_val_physical
     | intros Hfail;
       wp_finish
     | intros Hsuc;
