theories/language/rules.v
@@ -17,25 +17,21 @@ From zebre Require Import
   options.
 
 Implicit Types l : loc.
-Implicit Types p : prophecy_id.
 Implicit Types lit : literal.
 Implicit Types e : expr.
 Implicit Types es : list expr.
 Implicit Types v w : val.
 Implicit Types σ : state.
-Implicit Types κ : list observation.
 
 Section zebre_G.
   Context `{zebre_G : !ZebreG Σ}.
 
   Lemma base_reducible_equal v1 v2 σ :
-    val_physical v1 →
-    val_physical v2 →
     base_reducible (v1 = v2) σ.
   Proof.
     destruct
-      v1 as [[b1 | i1 | l1 | |] | | tag1 []],
-      v2 as [[b2 | i2 | l2 | |] | | tag2 []].
+      v1 as [[b1 | i1 | l1] | | tag1 []],
+      v2 as [[b2 | i2 | l2] | | tag2 []].
     all:
       try first
       [ destruct (decide (b1 = b2)); first subst
@@ -46,8 +42,6 @@ Section zebre_G.
     all: auto with zebre.
   Qed.
   Lemma wp_equal v1 v2 E Φ :
-    val_physical v1 →
-    val_physical v2 →
     ▷ (
       ( ⌜val_neq v1 v2⌝ -∗
         Φ #false
@@ -58,13 +52,13 @@ Section zebre_G.
     ) ⊢
     WP v1 = v2 @ E {{ Φ }}.
   Proof.
-    iIntros "% % HΦ".
-    iApply wp_lift_atomic_base_step_no_fork; first done. iIntros "%σ1 %ns %κ %κ' %nt (Hσ & Hκ) !>".
+    iIntros "HΦ".
+    iApply wp_lift_atomic_base_step_no_fork; first done. iIntros "%σ1 %ns %κ %κ' %nt Hσ !>".
     iSplit. { iPureIntro. apply base_reducible_equal; done. }
     iIntros "%e2 %σ2 %es %Hstep !> _".
     destruct
-      v1 as [[b1 | i1 | l1 | |] | | tag1 []],
-      v2 as [[b2 | i2 | l2 | |] | | tag2 []].
+      v1 as [[b1 | i1 | l1] | | tag1 []],
+      v2 as [[b2 | i2 | l2] | | tag2 []].
     all:
       try first
       [ destruct (decide (b1 = b2)); first subst
@@ -112,7 +106,7 @@ Section zebre_G.
     }}}.
   Proof.
     iIntros (Hlen <-%of_to_vals) "%Φ _ HΦ".
-    iApply wp_lift_atomic_base_step_no_fork; first done. iIntros "%σ1 %ns %κ %κ' %nt (Hσ1 & Hκ) !>".
+    iApply wp_lift_atomic_base_step_no_fork; first done. iIntros "%σ1 %ns %κ %κ' %nt Hσ1 !>".
     iSplit; first auto with zebre. iIntros "!> %e2 %σ2 %es %Hstep _".
     invert_base_step. rename select (list val) into vs.
     iStep. iFrame.
@@ -135,7 +129,7 @@ Section zebre_G.
     }}}.
   Proof.
     iIntros "%Hn %Φ _ HΦ".
-    iApply wp_lift_atomic_base_step_no_fork; first done. iIntros "%σ1 %ns %κ %κ' %nt (Hσ1 & Hκ) !>".
+    iApply wp_lift_atomic_base_step_no_fork; first done. iIntros "%σ1 %ns %κ %κ' %nt Hσ1 !>".
     iSplit; first auto with zebre. iIntros "!> %e2 %σ2 %es %Hstep _".
     invert_base_step.
     iStep. iFrame.
@@ -171,7 +165,7 @@ Section zebre_G.
     }}}.
   Proof.
     iIntros "%Φ >Hl HΦ".
-    iApply wp_lift_atomic_base_step_no_fork; first done. iIntros "%σ1 %ns %κ %κ' %nt (Hσ & Hκ) !>".
+    iApply wp_lift_atomic_base_step_no_fork; first done. iIntros "%σ1 %ns %κ %κ' %nt Hσ !>".
     iDestruct (gen_heap_valid with "Hσ Hl") as %Hlookup.
     iSplit; first eauto with zebre. iIntros "%e2 %σ2 %es %Hstep !> _".
     invert_base_step.
@@ -189,7 +183,7 @@ Section zebre_G.
     }}}.
   Proof.
     iIntros "%Φ >Hl HΦ".
-    iApply wp_lift_atomic_base_step_no_fork; first done. iIntros "%σ1 %ns %κ %κ' %nt (Hσ & Hκ) !>".
+    iApply wp_lift_atomic_base_step_no_fork; first done. iIntros "%σ1 %ns %κ %κ' %nt Hσ !>".
     iDestruct (gen_heap_valid with "Hσ Hl") as %Hlookup.
     iSplit; first eauto with zebre. iIntros "%e2 %σ2 %es %Hstep !> _".
     invert_base_step.
@@ -208,7 +202,7 @@ Section zebre_G.
     }}}.
   Proof.
     iIntros "%Φ >Hl HΦ".
-    iApply wp_lift_atomic_base_step_no_fork; first done. iIntros "%σ1 %ns %κ %κ' %nt (Hσ & Hκ) !>".
+    iApply wp_lift_atomic_base_step_no_fork; first done. iIntros "%σ1 %ns %κ %κ' %nt Hσ !>".
     iDestruct (gen_heap_valid with "Hσ Hl") as %Hlookup.
     iSplit; first eauto with zebre. iIntros "%e2 %σ2 %es %Hstep !> _".
     invert_base_step.
@@ -217,15 +211,13 @@ Section zebre_G.
   Qed.
 
   Lemma base_reducible_cas l v v1 v2 σ :
-    σ.(state_heap) !! l = Some v →
-    val_physical v →
-    val_physical v1 →
+    σ !! l = Some v →
     base_reducible (Cas #l v1 v2) σ.
   Proof.
     intros.
     destruct
-      v as [[b | i | l' | |] | | tag []],
-      v1 as [[b1 | i1 | l1 | |] | | tag1 []].
+      v as [[b | i | l'] | | tag []],
+      v1 as [[b1 | i1 | l1] | | tag1 []].
     all:
       try first
       [ destruct (decide (b = b1)); first subst
@@ -236,8 +228,6 @@ Section zebre_G.
     all: eauto with zebre.
   Qed.
   Lemma wp_cas l dq v v1 v2 E Φ :
-    val_physical v →
-    val_physical v1 →
     ▷ l ↦{dq} v -∗
     ▷ (
       ( ⌜val_neq v v1⌝ -∗
@@ -255,15 +245,15 @@ Section zebre_G.
     ) -∗
     WP Cas #l v1 v2 @ E {{ Φ }}.
   Proof.
-    iIntros "% % >Hl HΦ".
-    iApply wp_lift_atomic_base_step_no_fork; first done. iIntros "%σ1 %ns %κ %κ' %nt (Hσ & Hκ) !>".
+    iIntros ">Hl HΦ".
+    iApply wp_lift_atomic_base_step_no_fork; first done. iIntros "%σ1 %ns %κ %κ' %nt Hσ !>".
     iDestruct (gen_heap_valid with "Hσ Hl") as %Hlookup.
 
     iSplit. { iPureIntro. eapply base_reducible_cas; done. }
     iIntros "%e2 %σ2 %es %Hstep !> _".
     destruct
-      v as [[b | i | l' | |] | | tag []],
-      v1 as [[b1 | i1 | l1 | |] | | tag1 []].
+      v as [[b | i | l'] | | tag []],
+      v1 as [[b1 | i1 | l1] | | tag1 []].
     all:
       try first
       [ destruct (decide (b = b1)); first subst
@@ -287,8 +277,6 @@ Section zebre_G.
       end.
   Qed.
   Lemma wp_cas_literal l dq lit lit1 v2 E Φ :
-    literal_physical lit →
-    literal_physical lit1 →
     ▷ l ↦{dq} #lit -∗
     ▷ (
       ( ⌜lit ≠ lit1⌝ -∗
@@ -306,14 +294,13 @@ Section zebre_G.
     ) -∗
     WP Cas #l #lit1 v2 @ E {{ Φ }}.
   Proof.
-    iIntros "% % >Hl HΦ".
+    iIntros ">Hl HΦ".
     iApply (wp_cas with "Hl"); [done.. |].
     iSplit.
     - iDestruct "HΦ" as "($ & _)".
     - iDestruct "HΦ" as "(_ & $)".
   Qed.
   Lemma wp_cas_suc l lit lit1 v2 E :
-    literal_physical lit →
     lit = lit1 →
     {{{
       ▷ l ↦ #lit
@@ -324,7 +311,7 @@ Section zebre_G.
       l ↦ v2
     }}}.
   Proof.
-    iIntros (Hlit ->) "%Φ >Hl HΦ".
+    iIntros (->) "%Φ >Hl HΦ".
     iApply (wp_cas_literal with "Hl"); [done.. |].
     iSteps.
   Qed.
@@ -340,7 +327,7 @@ Section zebre_G.
     }}}.
   Proof.
     iIntros "%Φ >Hl HΦ".
-    iApply wp_lift_atomic_base_step_no_fork; first done. iIntros "%σ1 %ns %κ %κ' %nt (Hσ & Hκ) !>".
+    iApply wp_lift_atomic_base_step_no_fork; first done. iIntros "%σ1 %ns %κ %κ' %nt Hσ !>".
     iDestruct (gen_heap_valid with "Hσ Hl") as %Hlookup.
     iSplit; first eauto with zebre. iIntros "%e2 %σ2 %es %Hstep !> _".
     invert_base_step.
@@ -354,102 +341,9 @@ Section zebre_G.
     WP Fork e @ E {{ Φ }}.
   Proof.
     iIntros "Hwp HΦ".
-    iApply wp_lift_atomic_base_step; first done. iIntros "%σ1 %ns %κ %κ' %nt (Hσ1 & Hκ) !>".
+    iApply wp_lift_atomic_base_step; first done. iIntros "%σ1 %ns %κ %κ' %nt Hσ1 !>".
     iSplit; first auto with zebre. iIntros "!> %v2 %σ2 %es %Hstep _".
     invert_base_step.
     iFrame. iSteps.
-  Qed.
-
-  Lemma wp_proph E :
-    {{{ True }}}
-      Proph @ E
-    {{{ pvs p,
-      RET #p;
-      proph p pvs
-    }}}.
-  Proof.
-    iIntros "%Φ _ HΦ".
-    iApply wp_lift_atomic_base_step_no_fork; first done. iIntros "%σ1 %ns %κ %κ' %nt (Hσ & Hκ) !>".
-    iSplit; first eauto with zebre. iIntros "%e2 %σ2 %es %Hstep !> _".
-    invert_base_step.
-    iMod (proph_map_new_proph p with "Hκ") as "(Hκ & Hp)"; first done.
-    iFrame. iSteps.
-  Qed.
-
-  Lemma resolve_reducible e σ p v :
-    Atomic StronglyAtomic e →
-    reducible e σ →
-    reducible (Resolve e #p v) σ.
-  Proof.
-    intros A (κ & e' & σ' & es & H).
-    exists (κ ++ [(p, (default v (to_val e'), v))]), e', σ', es.
-    eapply (Ectx_step []); try done.
-    assert (∃ w, Val w = e') as (w & <-).
-    { unfold Atomic in A. apply (A σ e' κ σ' es) in H. unfold is_Some in H.
-      destruct H as [w H]. exists w. simpl in H. by apply (of_to_val _ _ H).
-    }
-    simpl. constructor. by apply prim_step_to_val_is_base_step.
-  Qed.
-  Lemma step_resolve e v1 v2 σ1 κ e2 σ2 es :
-    Atomic StronglyAtomic e →
-    prim_step (Resolve e v1 v2) σ1 κ e2 σ2 es →
-    base_step (Resolve e v1 v2) σ1 κ e2 σ2 es.
-  Proof.
-    intros A [K e1' e2' Hfill -> step]. simpl in *.
-    induction K as [| k K _] using rev_ind.
-    + simpl in *. subst. invert_base_step. constructor. done.
-    + rewrite fill_app /= in Hfill. destruct k; inversion Hfill; subst; clear Hfill.
-      - assert (fill_item k (fill K e1') = fill (K ++ [k]) e1') as Heq1; first by rewrite fill_app.
-        assert (fill_item k (fill K e2') = fill (K ++ [k]) e2') as Heq2; first by rewrite fill_app.
-        rewrite fill_app /=. rewrite Heq1 in A.
-        assert (is_Some (to_val (fill (K ++ [k]) e2'))) as H.
-        { eapply (A σ1 _ κ σ2 es), (Ectx_step (K ++ [k])); done. }
-        destruct H as [v H]. apply to_val_fill_some in H. destruct H, K; done.
-      - rename select (of_val v1 = _) into Hv1.
-        assert (to_val (fill K e1') = Some v1) as Hfill_v1 by rewrite -Hv1 //.
-        apply to_val_fill_some in Hfill_v1 as (-> & ->).
-        invert_base_step.
-      - rename select (of_val v2 = _) into Hv2.
-        assert (to_val (fill K e1') = Some v2) as Hfill_v2 by rewrite -Hv2 //.
-        apply to_val_fill_some in Hfill_v2 as (-> & ->).
-        invert_base_step.
-  Qed.
-  Lemma wp_resolve e p v pvs E Φ :
-    Atomic StronglyAtomic e →
-    to_val e = None →
-    proph p pvs -∗
-    WP e @ E {{ res,
-      ∀ pvs',
-      ⌜pvs = (res, v) :: pvs'⌝ -∗
-      proph p pvs' -∗
-      Φ res
-    }} -∗
-    WP Resolve e #p v @ E {{ Φ }}.
-  Proof.
-    iIntros "%Hatomic %He Hp Hwp".
-    rewrite !wp_unfold /wp_pre /= He. simpl in *.
-    iIntros "%σ1 %ns %κ %κ' %nt (Hσ & Hκ)".
-    destruct κ as [| (p' & (w' & v')) κ'' _] using rev_ind.
-    - iMod ("Hwp" $! σ1 ns [] κ' nt with "[$Hσ $Hκ]") as "(%Hreducible & Hwp)".
-      iSplitR. { iPureIntro. apply resolve_reducible; done. }
-      iIntros "!> %e2 %σ2 %es %Hstep".
-      exfalso. apply step_resolve in Hstep; last done.
-      invert_base_step.
-      destruct κ; done.
-    - rewrite -assoc.
-      iMod ("Hwp" $! σ1 ns _ _ nt with "[$Hσ $Hκ]") as "(%Hreducible & Hwp)".
-      iSplitR. { iPureIntro. apply resolve_reducible; done. }
-      iIntros "!> %e2 %σ2 %es %Hstep H£".
-      apply step_resolve in Hstep; last done.
-      invert_base_step. simplify_list_eq.
-      iMod ("Hwp" $! (Val w') σ2 es with "[%] H£") as "Hwp".
-      { eexists [] _ _; done. }
-      do 2 iModIntro.
-      iMod "Hwp" as "Hwp".
-      iApply (step_fupdN_wand with "Hwp"). iIntros "!> > (($ & Hκ) & Hwp)".
-      iMod (proph_map_resolve_proph p' (w', v') κ' with "[$Hκ $Hp]") as (vs' ->) "($ & Hp')".
-      rewrite !wp_unfold /wp_pre /=.
-      iDestruct "Hwp" as "(HΦ & $)".
-      iSteps.
   Qed.
 End zebre_G.
