theories/language/typeclass_instances.v
@@ -114,31 +114,6 @@ Section atomic.
   Proof.
     solve_atomic.
   Qed.
-
-  #[global] Instance proph_atomic a :
-    Atomic a Proph.
-  Proof.
-    solve_atomic.
-  Qed.
-  #[global] Instance resolve_atomic a e v1 v2 :
-    Atomic a e →
-    Atomic a (Resolve e (Val v1) (Val v2)).
-  Proof.
-    rename e into e1. intros H σ1 e2 κ σ2 es [K e1' e2' Hfill -> step].
-    simpl in *. induction K as [| k K _] using rev_ind; simpl in Hfill.
-    - subst. inversion_clear step. by eapply (H σ1 (Val _) _ σ2 es), base_prim_step.
-    - rewrite fill_app. rewrite fill_app in Hfill.
-      assert (∀ v, Val v = fill K e1' → False) as fill_absurd.
-      { intros v Hv. assert (to_val (fill K e1') = Some v) as Htv by by rewrite -Hv.
-        apply to_val_fill_some in Htv. destruct Htv as [-> ->]. inversion step. }
-      destruct k; (inversion Hfill; clear Hfill; subst; try
-        match goal with | H : Val ?v = fill K e1' |- _ => by apply fill_absurd in H end).
-      refine (_ (H σ1 (fill (K ++ [_]) e2') _ σ2 es _)).
-      + destruct a; intro Hs; simpl in *.
-        * destruct Hs as [v Hs]. apply to_val_fill_some in Hs. by destruct Hs, K.
-        * apply irreducible_resolve. by rewrite fill_app in Hs.
-      + econstructor; try done. simpl. by rewrite fill_app.
-  Qed.
 End atomic.
 
 Class AsValRec v f x e :=
