theories/persistent/base.v
@@ -1,6 +1,0 @@
-From zebre Require Import
-  prelude.
-From zebre.language Require Export
-  rules.
-From zebre Require Import
-  options.
